systemf: simplify the calculus by removing some features we do not need; show that semantic typing implies type safety

theories/type_systems/systemf/bigstep.v
@@ -1,7 +1,6 @@
 From stdpp Require Import gmap base relations.
 From ffpl.lib Require Import prelude.
-From ffpl.lib Require Export debruijn.
-From ffpl.type_systems.systemf Require Import lang notation.
+From ffpl.type_systems.systemf Require Import lang notation deterministic.
 From Equations Require Import Equations.
 
 (** * Big-step semantics *)
@@ -20,10 +19,6 @@ Inductive big_step : expr -> val -> Prop :=
       big_step e2 v2 ->
       bin_op_eval op v1 v2 = Some v' ->
       big_step (BinOp op e1 e2) v'
-  | bs_unop e v v' op :
-      big_step e v ->
-      un_op_eval op v = Some v' ->
-      big_step (UnOp op e) v'
   | bs_app e1 e2 e v2 v :
       big_step e1 (LamV e) ->
       big_step e2 v2 ->
@@ -60,20 +55,6 @@ Inductive big_step : expr -> val -> Prop :=
   | bs_snd e v1 v2 :
       big_step e (v1, v2) ->
       big_step (Snd e) v2
-  | bs_injl e v :
-      big_step e v ->
-      big_step (InjL e) (InjLV v)
-  | bs_injr e v :
-      big_step e v ->
-      big_step (InjR e) (InjRV v)
-  | bs_casel e e1 e2 v v' :
-      big_step e (InjLV v) ->
-      big_step (e1 (of_val v)) v' ->
-      big_step (Case e e1 e2) v'
-  | bs_caser e e1 e2 v v' :
-      big_step e (InjRV v) ->
-      big_step (e2 (of_val v)) v' ->
-      big_step (Case e e1 e2) v'
     .
 #[export] Hint Constructors big_step : core.
 
@@ -95,27 +76,13 @@ Qed.
 
 (** ** Big-step semantics implies contextual semantics *)
 
-(** This is mostly a sanity check. It is also rather tedious for languages
-with as many cases as ours. *)
-
-Lemma fill_rtc_contextual_step {e1 e2} K :
-  rtc contextual_step e1 e2 ->
-  rtc contextual_step (fill K e1) (fill K e2).
-Proof.
-  induction 1 as [ | x y z H1 H2 IH]; first done.
-  etrans; last apply IH.
-  econstructor 2; last constructor 1.
-  by apply fill_contextual_step.
-Qed.
-
 Lemma big_step_contextual e v :
   big_step e v -> rtc contextual_step e (of_val v).
 Proof.
-  induction 1 as [ | | e1 e2 v1 v2 v' op H1 IH1 H2 IH2 Hop | e v v' op H1 IH1 Hop
+  induction 1 as [ | | e1 e2 v1 v2 v' op H1 IH1 H2 IH2 Hop
     | e1 e2 e v2 v H1 IH1 H2 IH2 H3 IH3 | e1 e2 v1 H1 IH1 H2 IH2 | |
     | e1 e2 v1 v2 H1 IH1 H2 IH2 | e0 e1 e2 v H1 IH1 H2 IH2 | e0 e1 e2 v H1 IH1 H2 IH2
-    | e1 e2 v1 v2 H1 IH1 H2 IH2 | e v1 v2 H IH | e v1 v2 H IH | e v H IH | e v H IH
-    | e e1 e2 v v' H1 IH1 H2 IH2 | e e1 e2 v v' H1 IH1 H2 IH2 ].
+    | e1 e2 v1 v2 H1 IH1 H2 IH2 | e v1 v2 H IH | e v1 v2 H IH ].
   - constructor.
   - constructor.
   - (* binop *)
@@ -125,15 +92,6 @@ Proof.
     { eapply (fill_rtc_contextual_step (BinOpLCtx _ HoleCtx _)). done. }
     simpl.
     etrans.
-    { econstructor 2; last econstructor 1.
-      apply base_contextual_step. econstructor; last done.
-      all: apply to_of_val.
-    }
-    constructor.
-  - (* unop *)
-    etrans.
-    { eapply (fill_rtc_contextual_step (UnOpCtx _ HoleCtx)). done. }
-    simpl. etrans.
     { econstructor 2; last econstructor 1.
       apply base_contextual_step. econstructor; last done.
       all: apply to_of_val.
@@ -188,20 +146,19 @@ Proof.
     econstructor.
     { eapply base_contextual_step. simpl. eauto.  }
     econstructor.
-  - etrans.
-    { eapply (fill_rtc_contextual_step (InjLCtx HoleCtx)). done. }
-    econstructor.
-  - etrans.
-    { eapply (fill_rtc_contextual_step (InjRCtx HoleCtx)). done. }
-    econstructor.
-  - etrans.
-    { eapply (fill_rtc_contextual_step (CaseCtx HoleCtx e1 e2)). done. }
-    simpl. econstructor.
-    { eapply base_contextual_step. eauto.  }
-    done.
-  - etrans.
-    { eapply (fill_rtc_contextual_step (CaseCtx HoleCtx e1 e2)). done. }
-    simpl. econstructor.
-    { eapply base_contextual_step. eauto. }
-    done.
+Qed.
+
+(** Together with determinism, this means big-step captures all the program behaviors:
+any execution that start at [e] can be completed to go to [v]. *)
+Lemma big_step_complete {e e' v} :
+  big_step e v ->
+  rtc contextual_step e e' ->
+  rtc contextual_step e' (of_val v).
+Proof.
+  intros Heval%big_step_contextual Hsteps.
+  destruct (contextual_steps_det Heval Hsteps) as [Hsteps'|Hsteps'].
+  - inversion Hsteps'; simplify_eq/=; first done.
+    exfalso. eapply conextual_step_no_val; first done.
+    eapply is_val_of_val. done.
+  - done.
 Qed.
