theories/type_systems/systemf/deterministic.v
@@ -1,0 +1,79 @@
+From stdpp Require Import gmap base relations.
+From ffpl.lib Require Import prelude.
+From ffpl.type_systems.systemf Require Import lang notation.
+From Equations Require Import Equations.
+
+(** Proof that our small-step semantics are deterministic. *)
+
+Lemma base_step_det e e1 e2 :
+  base_step e e1 -> base_step e e2 -> e1 = e2.
+Proof.
+  inversion 1; inversion 1; subst; congruence.
+Qed.
+
+(** We need this very technical lemma with tons of cases. None of the cases is
+very interesting. We use some Coq tactic programming to handle them all
+automatically. *)
+
+Lemma base_redex_unique K1 e1 e1' K2 e2 e2' :
+  fill K1 e1 = fill K2 e2 ->
+  base_step e1 e1' ->
+  base_step e2 e2' ->
+  K1 = K2 /\ e1 = e2.
+Proof.
+  induction K1 in K2, e2, e2' |- *; simpl.
+  all: destruct K2; intros; simplify_eq/=.
+  all: repeat match goal with
+      | H : ?e' = fill ?K ?e |- _ =>
+          (* maybe [e'] is a value *)
+          let Hval := fresh "Hval" in
+          assert (is_val e') as Hval by (by eauto);
+          rewrite H in Hval;
+          clear H (* avoid loops *)
+      | H : fill ?K ?e = of_val _ |- _ =>
+          symmetry in H (* make it hit the case above *)
+      | H : is_val (fill _ _) |- _ =>
+          apply fill_is_val_inv in H
+      | H : to_val (fill _ _) = Some _ |- _ =>
+          apply is_val_to_val in H
+      | H1 : is_val ?e, H2 : base_step ?e _ |- _ =>
+          apply base_step_no_val in H2; done
+      | H : fill _ ?e1 = fill _ ?e2, H1 : base_step ?e1 _, H2 : base_step ?e2 _ |- _ =>
+          destruct (IHK1 _ _ _ H H1 H2); simplify_eq/=; by eauto
+      | H : base_step _ _ |- _ =>
+          inversion H;
+          simplify_eq/=;
+          [clear H] (* also asserts that there is exactly one goal *)
+      | H : base_step _ _ |- _ =>
+          inversion H;
+          simplify_eq/=;
+          done (* sometimes this closes all goals *)
+      | H : base_step _ _ |- _ =>
+          inversion H;
+          simplify_eq/=;
+          [clear H|clear H] (* for if, we need to allow 2 goals *)
+      end.
+Qed.
+
+Lemma contextual_step_det {e e1 e2} :
+  contextual_step e e1 -> contextual_step e e2 -> e1 = e2.
+Proof.
+  inversion 1; inversion 1; subst.
+  edestruct base_redex_unique; [done|done|done|subst].
+  f_equal. eapply base_step_det; done.
+Qed.
+
+(** It follows that if [e] can step to two different terms, then
+really one is just a more reduced form of the other. *)
+Lemma contextual_steps_det {e e1 e2} :
+  rtc contextual_step e e1 ->
+  rtc contextual_step e e2 ->
+  (rtc contextual_step e1 e2 \/ rtc contextual_step e2 e1).
+Proof.
+  induction 1 as [e|e e1 e1' Hstep1 Hsteps1 IH] in e2 |- *.
+  { eauto. }
+  destruct 1 as [e|e e2 e2' Hstep2 Hsteps2].
+  { right. econstructor; done. }
+  pose proof (contextual_step_det Hstep1 Hstep2) as ->.
+  eapply IH. done.
+Qed.
